theories/LogicalRelation/Weakening.v
@@ -1,6 +1,6 @@
 From LogRel.AutoSubst Require Import core unscoped Ast Extra.
 From LogRel Require Import Notations Utils BasicAst LContexts Context NormalForms UntypedValues Weakening GenericTyping Monad LogicalRelation DeclarativeInstance.
-From LogRel.LogicalRelation Require Import Induction Irrelevance Transitivity Escape.
+From LogRel.LogicalRelation Require Import Induction Irrelevance Reflexivity Transitivity Escape.
 
 Set Universe Polymorphism.
 
@@ -222,42 +222,138 @@ Lemma wkEq@{i j k l} {wl Γ Δ A B l} (ρ : Δ ≤ Γ) (wfΔ : [|-Δ]< wl >) (lr
     now eapply WRedEq.
   Qed.
 
-  
+  Lemma isLRFun_ren : forall wl Γ Δ t A l (ρ : Δ ≤ Γ) (wfΔ : [|- Δ]< wl >) (ΠA : [Γ ||-Π< l > A]< wl >),
+    isLRFun ΠA t -> isLRFun (wkΠ ρ wfΔ ΠA) t⟨ρ⟩.
+  Proof.
+    intros * [A' t' Htree Hdom Ht|]; [unshelve econstructor 1 | ] ; fold ren_term.
+    - intros Ξ k' ? ρ' f * ha; cbn.
+      eapply DTree_fusion.
+      + eapply (Htree _ _ a (ρ' ∘w ρ) f Hd).
+        irrelevance.
+      + eapply (PolyRed.posTree ΠA (ρ' ∘w ρ) f Hd).
+        irrelevance.
+    - intros Ξ wl' ρ' f *; cbn.
+      assert (eq : forall t, t⟨ρ' ∘w ρ⟩ = t⟨ρ⟩⟨ρ'⟩) by now bsimpl.
+      irrelevance0 ; [apply eq| ].
+      assert (eq' : forall t, t⟨ρ' ∘w ρ⟩ = (ren_term ρ t)⟨ρ'⟩) by now bsimpl.
+      rewrite <- eq'.
+      now unshelve eapply Hdom.
+    - intros Ξ wl' a ρ' f wfΞ ha wl'' Ho Ho'; cbn in *.
+      assert (eq : forall t, t⟨ρ' ∘w ρ⟩ = t⟨ρ⟩⟨ρ'⟩) by now bsimpl.
+      unshelve eassert (Ht0 := Ht Ξ wl' a (ρ' ∘w ρ) f wfΞ _ wl'' (over_tree_fusion_r Ho') (over_tree_fusion_l Ho')).
+      replace ((ren_term (upRen_term_term ρ) t')[a .: ρ' >> tRel]) with (t'[a .: (ρ' ∘w ρ) >> tRel]) by now bsimpl.
+      irrelevance0; [|apply Ht0].
+      now bsimpl.
+    - constructor.
+      change [Δ |- f⟨ρ⟩ ~ f⟨ρ⟩ : (tProd (PiRedTy.dom ΠA) (PiRedTy.cod ΠA))⟨ρ⟩]< wl >.
+      now eapply convneu_wk.
+  Qed.
+
   (* TODO: use program or equivalent to have only the first field non-opaque *)
   Lemma wkΠTerm {wl Γ Δ u A l} (ρ : Δ ≤ Γ) (wfΔ : [|- Δ]< wl >) (ΠA : [Γ ||-Π< l > A]< wl >) 
-    (ΠA' := wkΠ' ρ wfΔ ΠA) : 
-    [Γ||-Π u : A | PiRedTyPack.toPiRedTy ΠA]< wl > -> 
-    [Δ ||-Π u⟨ρ⟩ : A⟨ρ⟩ | PiRedTyPack.toPiRedTy ΠA' ]< wl >.
+    (ΠA' := wkΠ ρ wfΔ ΠA) : 
+    [Γ||-Π u : A | ΠA]< wl > -> 
+    [Δ ||-Π u⟨ρ⟩ : A⟨ρ⟩ | ΠA' ]< wl >.
   Proof.
-    intros [t]. 
-    unshelve econstructor ;  try change (tProd _ _) with ((PiRedTyPack.prod ΠA)⟨ρ⟩).
-    - exact (t⟨ρ⟩).
-    - exact redN.
-    - intros ; unshelve eapply appN ; try assumption.
-      exact (ρ0 ∘w ρ).
-      subst ΠA'. 
-      irrelevance.
+    intros [t].
+    unshelve econstructor ; [exact (t⟨ρ⟩) | ..].
+    all: try change (tProd _ _) with (ΠA.(outTy)⟨ρ⟩).
+    - intros ?? a ρ' f ??.
+      eapply DTree_fusion ; [apply (appTree _ _ a (ρ' ∘w ρ) f Hd) | eapply (PolyRed.posTree ΠA (ρ' ∘w ρ) f Hd)].
+      all: irrelevance0 ; [ | eassumption] .
+      all: subst ΠA'; bsimpl; try rewrite scons_comp'; reflexivity.
     - now eapply redtmwf_wk.
-    - apply isFun_ren; assumption.
-    - now apply tm_nf_wk.
-    - eapply convtm_wk; eassumption.
-    - intros ? a ? ρ' * ?.
+    - now apply convtm_wk.
+    - now apply isLRFun_ren.
+    - intros ? a wl' ρ' f ?? wl'' Ho Ho' ; cbn in *.
       replace ((t ⟨ρ⟩)⟨ ρ' ⟩) with (t⟨ρ' ∘w ρ⟩) by now bsimpl.
       irrelevance0.
-      2: unshelve eapply app;  [exact l'|..]; subst ΠA'; try irrelevance ; assumption. 
-      subst ΠA'; bsimpl; try rewrite scons_comp'; reflexivity.
-    - intros ???? ρ' ???????????.
+      2: unshelve apply app ; [| | eassumption| subst ΠA'; irrelevance |..] ; auto. 
+      + subst ΠA'; bsimpl; try rewrite scons_comp'; reflexivity.
+      + now eapply over_tree_fusion_r.
+      + now eapply over_tree_fusion_l.
+    - intros ??? wl' ρ' f ??????? ; cbn in *.
       replace ((t ⟨ρ⟩)⟨ ρ' ⟩) with (t⟨ρ' ∘w ρ⟩) by now bsimpl.
       irrelevance0.
-      2: unshelve eapply eq;  [exact l'|..]; subst ΠA'; try irrelevance ; assumption.
-      subst ΠA'; bsimpl; try rewrite scons_comp'; reflexivity.
+      2: unshelve apply eq; [| | eassumption|..] ; auto ; try (subst ΠA'; irrelevance).
+      + subst ΠA'; bsimpl; try rewrite scons_comp'; reflexivity.
+      + now eapply over_tree_fusion_r.
+      + now eapply over_tree_fusion_l.
   Defined.
+
 
   Lemma wkNeNf {wl Γ Δ k A} (ρ : Δ ≤ Γ) (wfΔ : [|-Δ]< wl >) : 
     [Γ ||-NeNf k : A]< wl > -> [Δ ||-NeNf k⟨ρ⟩ : A⟨ρ⟩]< wl >.
   Proof.
-    intros []; constructor. 1:apply tm_ne_wk. all: gen_typing.
+    intros []; constructor. all: gen_typing.
   Qed.  
+
+
+  Lemma isLRPair_ren : forall wl Γ Δ t A l (ρ : Δ ≤ Γ) (wfΔ : [|- Δ]< wl >) (ΣA : [Γ ||-Σ< l > A]< wl >),
+    isLRPair ΣA t -> isLRPair (wkΣ ρ wfΔ ΣA) t⟨ρ⟩.
+  Proof.
+    assert (eq : forall Γ Δ Ξ (ρ : Δ ≤ Γ) (ρ' : Ξ ≤ Δ) t, t⟨ρ' ∘w ρ⟩ = t⟨ρ⟩⟨ρ'⟩) by now bsimpl.
+    intros * [A' B' a b Hdom codTree Hcod Hfst sndTree Hsnd|]; unshelve econstructor ; tea ; refold.
+    - refold; intros Ξ wl' a' ρ' f wfΞ ha'.
+      eapply DTree_fusion.
+      + unshelve eapply (codTree Ξ wl' a' (ρ' ∘w ρ) f wfΞ _).
+        irrelevance0 ; [symmetry | exact ha'].
+        now apply eq.
+      + unshelve eapply (PolyRed.posTree ΣA (ρ' ∘w ρ) f wfΞ).
+        2: irrelevance0 ; [symmetry | exact ha'].
+        now apply eq.
+    - refold; intros Ξ wl' ρ' f wfΞ ; cbn.
+      erewrite <- eq.
+      irrelevance0; [|now unshelve apply Hfst].
+      now bsimpl.
+    - intros Ξ wl' ρ' f wfΞ.
+      eapply DTree_fusion.
+      + unshelve eapply (sndTree _ _ (ρ' ∘w ρ)) ; now eauto.
+      + eapply (PolyRed.posTree ΣA (ρ' ∘w ρ) f wfΞ).
+        now eapply Hfst.
+    - intros Ξ wl' ρ' f wfΞ.
+      irrelevance0; [apply eq|].
+      rewrite <- eq.
+      now unshelve apply Hdom.
+    - intros Ξ wl' a' ρ' f wfΞ ha' wl'' Ho Ho'; cbn in *.
+      unshelve eassert (Hcod0 := Hcod Ξ wl' a' (ρ' ∘w ρ) f wfΞ _ wl'' _ (over_tree_fusion_l Ho')).
+      { exact (over_tree_fusion_r Ho'). }
+      replace (B'⟨upRen_term_term ρ⟩[a' .: ρ' >> tRel]) with B'[a' .: (ρ' ∘w ρ) >> tRel] by now bsimpl.
+      irrelevance0; [|apply Hcod0].
+      now bsimpl.
+    - refold; intros Ξ wl' ρ' f wfΞ wl'' Ho Ho' ; cbn in *.
+      rewrite <- (eq _ _ _ ρ ρ' b).
+      irrelevance0; [| unshelve apply (Hsnd _ _ _ f wfΞ)].
+      + now bsimpl.
+      + now eapply over_tree_fusion_r.
+      + now eapply over_tree_fusion_l.
+    - change [Δ |- p⟨ρ⟩ ~ p⟨ρ⟩ : (tSig (SigRedTy.dom ΣA) (SigRedTy.cod ΣA))⟨ρ⟩]< wl >.
+      now eapply convneu_wk.
+  Qed.
+
+  Lemma wkΣTerm {wl Γ Δ u A l} (ρ : Δ ≤ Γ) (wfΔ : [|- Δ]< wl >) (ΠA : [Γ ||-Σ< l > A]< wl >) 
+    (ΠA' := wkΣ ρ wfΔ ΠA) : 
+    [Γ||-Σ u : A | ΠA]< wl > -> 
+    [Δ ||-Σ u⟨ρ⟩ : A⟨ρ⟩ | ΠA' ]< wl >.
+  Proof.
+    intros [t]. 
+    unshelve eexists (t⟨ρ⟩) _ _; try (cbn; rewrite wk_sig).
+    - intros ?? ρ' f wfΔ'; rewrite wk_comp_ren_on; irrelevance0.
+      2: now unshelve eapply fstRed.
+      cbn; symmetry; apply wk_comp_ren_on.
+    - intros ?? ρ' f wfΔ' ; eapply DTree_fusion.
+      + now eapply (sndTree _ _ (ρ' ∘w ρ) f wfΔ') ; eauto.
+      + eapply (PolyRed.posTree ΠA (ρ' ∘w ρ) f wfΔ').
+        now eapply fstRed.
+    - now eapply redtmwf_wk.
+    - eapply convtm_wk; eassumption.
+    - apply isLRPair_ren; assumption.
+    - intros ? wl' ρ' f ? wl'' Ho Ho' ;  irrelevance0.
+      2: rewrite wk_comp_ren_on; unshelve eapply sndRed ; [ | eassumption | eassumption |.. ].
+      + rewrite <- wk_comp_ren_on; cbn; now rewrite <- wk_up_ren_subst.
+      + now eapply over_tree_fusion_r.
+      + now eapply over_tree_fusion_l.
+  Defined.
 
   Lemma wkTerm {wl Γ Δ t A l} (ρ : Δ ≤ Γ) (wfΔ : [|-Δ]< wl >) (lrA : [Γ ||-<l> A]< wl >) : 
     [Γ ||-<l> t : A | lrA]< wl > -> [Δ ||-<l> t⟨ρ⟩ : A⟨ρ⟩ | wk ρ wfΔ lrA]< wl >.
@@ -265,15 +361,14 @@ Lemma wkEq@{i j k l} {wl Γ Δ A B l} (ρ : Δ ≤ Γ) (wfΔ : [|-Δ]< wl >) (lr
     revert t Δ ρ wfΔ. pattern l, wl, Γ, A, lrA.
     eapply LR_rect_TyUr; clear l wl Γ A lrA.
     - intros ??????? ρ ? [te]; exists te⟨ρ⟩;  try change U with U⟨ρ⟩.
-      1, 4: gen_typing.
-      apply isType_ren; assumption.
-      now apply tm_nf_wk.
-      apply RedTyRecBwd ; apply wk; [assumption|]; now apply (RedTyRecFwd h).
+      + gen_typing.
+      + apply isType_ren; assumption.
+      + now apply convtm_wk.
+      + apply RedTyRecBwd ; apply wk; [assumption|]; now apply (RedTyRecFwd h).
     - intros ??????? ρ ? [te]. exists te⟨ρ⟩; cbn.
       + now eapply redtmwf_wk.
-      + apply tm_ne_wk; assumption.
-      + eapply convneu_wk; eassumption.
-    - intros ????? ihdom ihcod ?? ρ ?; apply wkΠTerm. 
+      + apply convneu_wk; assumption.
+    - intros; now apply wkΠTerm. 
     - intros ???? NA t ? ρ wfΔ; revert t; pose (NA' := wkNat ρ wfΔ NA).
       set (G := _); enough (h : G × (forall t, NatProp NA t -> NatProp NA' t⟨ρ⟩)) by apply h.
       subst G; apply NatRedInduction.
@@ -283,23 +378,45 @@ Lemma wkEq@{i j k l} {wl Γ Δ A B l} (ρ : Δ ≤ Γ) (wfΔ : [|-Δ]< wl >) (lr
       + intros; constructor. 
         change tNat with tNat⟨ρ⟩.
         now eapply wkNeNf.
-    - intros ???? NA t ? ρ wfΔ.
-      intros Ht ; induction Ht.
-      econstructor.
-      + change tBool with tBool⟨ρ⟩. gen_typing.
-      + change tBool with tBool⟨ρ⟩. gen_typing.
-      + clear red eq. inversion prop ; subst ; try now econstructor.
-          constructor.
+    - intros ???? NA t ? ρ wfΔ; revert t; pose (NA' := wkBool ρ wfΔ NA).
+      set (G := _); enough (h : G × (forall t, BoolProp NA t -> BoolProp NA' t⟨ρ⟩)) by apply h.
+      subst G ; split.
+      2:{ intros t Ht ; inversion Ht ; subst; econstructor.
           change tBool with tBool⟨ρ⟩.
-          now eapply wkNeNf.
-    - intros ???? NA t ? ρ wfΔ.
-      intro Ht ; induction Ht ; econstructor.
+          now eapply wkNeNf. }
+      intros t Ht. induction Ht. econstructor.
+      + change tBool with tBool⟨ρ⟩; gen_typing.
+      + change tBool with tBool⟨ρ⟩; gen_typing.
+      + destruct prop ; econstructor.
+        change tBool with tBool⟨ρ⟩.
+        now eapply wkNeNf.
+    - intros ???? NA t ? ρ wfΔ; revert t; pose (NA' := wkEmpty ρ wfΔ NA).
+      set (G := _); enough (h : G × (forall t, EmptyProp (k := wl) Γ t -> EmptyProp (k := wl) Δ t⟨ρ⟩)) by apply h.
+      subst G.
+      split.
+      2:{ intros t Ht. inversion Ht. subst. econstructor.
+          change tEmpty with tEmpty⟨ρ⟩.
+          now eapply wkNeNf. }
+      intros t Ht. induction Ht. econstructor.
       + change tEmpty with tEmpty⟨ρ⟩; gen_typing.
       + change tEmpty with tEmpty⟨ρ⟩; gen_typing.
-      + inversion prop ; subst ; econstructor.
+      + destruct prop. econstructor.
         change tEmpty with tEmpty⟨ρ⟩.
         now eapply wkNeNf.
+    - intros; now apply wkΣTerm. 
+    - intros * _ _ * [??? prop]; econstructor; unfold_id_outTy; cbn; rewrite ?wk_Id.
+      1: now eapply redtmwf_wk.
+      1: now eapply convtm_wk.
+      destruct prop.
+      2: constructor; unfold_id_outTy; cbn; rewrite wk_Id; now eapply wkNeNf.
+      assert [|-Γ]< wl > by (escape; gen_typing); constructor; cbn.
+      1: now eapply wft_wk.
+      1: now eapply ty_wk.
+      2,3: eapply (IA.(IdRedTy.tyKripkeTmEq) _ _ _ (idε _) (idε _)); [now rewrite wk_comp_runit| irrelevance].
+      eapply (IA.(IdRedTy.tyKripkeEq) _ _ _ (idε _) (idε _)); [now rewrite wk_comp_runit| irrelevance].
+      Unshelve. all: tea.
   Qed.
+
 
   Lemma WwkTerm@{i j k l} {wl Γ Δ t A l} (ρ : Δ ≤ Γ) (wfΔ : [|-Δ]< wl >)
     (lrA : WLogRel@{i j k l} l wl Γ A) : 
@@ -307,7 +424,7 @@ Lemma wkEq@{i j k l} {wl Γ Δ A B l} (ρ : Δ ≤ Γ) (wfΔ : [|-Δ]< wl >) (lr
     W[ Δ ||-< l > t⟨ρ⟩ : A⟨ρ⟩ | Wwk@{i j k l} ρ wfΔ lrA]< wl >.
   Proof.
     intros [].
-    exists WNTm.
+    exists WTTm.
     intros.
     eapply wkTerm.
     now eapply WRedTm.
@@ -317,17 +434,17 @@ Lemma wkEq@{i j k l} {wl Γ Δ A B l} (ρ : Δ ≤ Γ) (wfΔ : [|-Δ]< wl >) (lr
     [LogRelRec l| Γ ||-U t : A | h ]< wl > -> [LogRelRec l | Δ||-U t⟨ρ⟩ : A⟨ρ⟩ | wkU ρ wfΔ h]< wl >.
   Proof.
     intros [te]. exists te⟨ρ⟩; change U with U⟨ρ⟩.
-    1, 4: gen_typing.
-    apply isType_ren; assumption.
-    now apply tm_nf_wk.
-    destruct l; [destruct (elim (URedTy.lt h))|cbn].
-    eapply (wk (l:=zero)); eassumption.
+    - gen_typing.
+    - apply isType_ren; assumption.
+    - now apply convtm_wk.
+    - destruct l; [destruct (elim (URedTy.lt h))|cbn].
+      eapply (wk (l:=zero)); eassumption.
   Defined.
 
   Lemma wkNeNfEq {wl Γ Δ k k' A} (ρ : Δ ≤ Γ) (wfΔ : [|-Δ]< wl >) : 
     [Γ ||-NeNf k ≅ k' : A]< wl > -> [Δ ||-NeNf k⟨ρ⟩ ≅ k'⟨ρ⟩ : A⟨ρ⟩]< wl >.
   Proof.
-    intros []; constructor. 1,2: apply tm_ne_wk. all: gen_typing.
+    intros []; constructor. gen_typing.
   Qed.  
 
   Lemma wkTermEq {wl Γ Δ t u A l} (ρ : Δ ≤ Γ) (wfΔ : [|-Δ]< wl >) (lrA : [Γ ||-<l> A]< wl >) : 
@@ -347,23 +464,24 @@ Lemma wkEq@{i j k l} {wl Γ Δ A B l} (ρ : Δ ≤ Γ) (wfΔ : [|-Δ]< wl >) (lr
     - intros ???????? ρ ? [tL tR].
       exists (tL⟨ρ⟩) (tR⟨ρ⟩); cbn.
       1,2: now eapply redtmwf_wk. 
-      1,2: apply tm_ne_wk; assumption.
       now eapply convneu_wk.
-    - intros ???? ΠA ihdom ihcod t u ? ρ ? [redL redR].
-      rewrite wkΠ_eq. set (X := wkΠ' _ _).
-      unshelve econstructor; try change (tProd _ _) with ((PiRedTyPack.prod ΠA)⟨ρ⟩).
+    - intros * ?? * []; rewrite wkΠ_eq. 
+      unshelve econstructor; cbn; try rewrite wk_prod.
       1,2: now eapply wkΠTerm.
-      + assumption.
-      + intros ; unshelve eapply eqappN ; try assumption.
-        exact (ρ0 ∘w ρ).
-        subst X. 
-        irrelevance.
+      + intros ? a ? ρ' * ? ; eapply DTree_fusion.
+        * unshelve eapply eqTree ; try assumption.
+          exact (ρ' ∘w ρ).
+          now irrelevance.
+        * eapply (PolyRed.posTree ΠA (ρ' ∘w ρ) f Hd).
+          now irrelevance.
       + now eapply convtm_wk.
       + intros ? a ? ρ' * ?. 
         replace (_ ⟨ ρ' ⟩) with (PiRedTm.nf redL) ⟨ρ' ∘w ρ⟩ by now bsimpl.
         replace (_ ⟨ ρ' ⟩) with (PiRedTm.nf redR) ⟨ρ' ∘w ρ⟩ by now bsimpl.
-        irrelevance0.  2: unshelve eapply eqApp; [exact l'|..]; subst X; try irrelevance ; assumption. 
-        subst X; bsimpl; now try rewrite scons_comp'.
+        irrelevance0.  2: unshelve eapply eqApp; [| exact f |..]; try irrelevance ; auto. 
+        * now rewrite <- wk_up_ren_subst.
+        * now eapply over_tree_fusion_r.
+        * now eapply over_tree_fusion_l.
     - intros ???? NA t u ? ρ wfΔ; revert t u; pose (NA' := wkNat ρ wfΔ NA).
       set (G := _); enough (h : G × (forall t u, NatPropEq NA t u -> NatPropEq NA' t⟨ρ⟩ u⟨ρ⟩)) by apply h.
       subst G; apply NatRedEqInduction.
@@ -389,5 +507,718 @@ Lemma wkEq@{i j k l} {wl Γ Δ A B l} (ρ : Δ ≤ Γ) (wfΔ : [|-Δ]< wl >) (lr
       + inversion prop ; subst ; econstructor.
         change tEmpty with tEmpty⟨ρ⟩.
         now eapply wkNeNfEq.
+    - intros * ?? * []; rewrite wkΣ_eq. 
+      unshelve econstructor; cbn; try rewrite wk_sig.
+      1,2: now eapply wkΣTerm.
+      + intros ? ? ρ' * ?? ; eapply DTree_fusion.
+        * unshelve eapply eqTree ; try assumption.
+          exact (ρ' ∘w ρ).
+        * eapply (PolyRed.posTree ΠA (ρ' ∘w ρ) f Hd).
+          eapply (redL.(SigRedTm.fstRed)).
+      + now eapply convtm_wk.
+      + intros; cbn; do 2 rewrite wk_comp_ren_on.
+        irrelevance0. 2: now unshelve eapply eqFst.
+        now rewrite wk_comp_ren_on.
+      + intros; cbn; irrelevance0.
+        2: do 2 rewrite wk_comp_ren_on; unshelve eapply (eqSnd _ _ _ f Hd).
+        * rewrite wk_comp_ren_on; now rewrite <- wk_up_ren_subst.
+        * now eapply over_tree_fusion_r.
+        * now eapply over_tree_fusion_l.
+    - intros * _ _ * [????? prop]; econstructor; unfold_id_outTy; cbn; rewrite ?wk_Id.
+      1,2: now eapply redtmwf_wk.
+      1: now eapply convtm_wk.
+      destruct prop.
+      2: constructor; unfold_id_outTy; cbn; rewrite wk_Id; now eapply wkNeNfEq.
+      assert [|-Γ]< wl > by (escape; gen_typing); constructor; cbn.
+      1,2: now eapply wft_wk.
+      1,2: now eapply ty_wk.
+      1,2:eapply (IA.(IdRedTy.tyKripkeEq) _ _ _ (idε _) (idε _)); [now rewrite wk_comp_runit| irrelevance].
+      all: eapply (IA.(IdRedTy.tyKripkeTmEq) _ _ _ (idε _) (idε _)); [now rewrite wk_comp_runit| irrelevance].
+      Unshelve. all: tea.
   Qed.
 End Weakenings.
+
+
+Section Red_Ltrans.
+  Context `{GenericTypingProperties}.
+  
+Lemma Id_Ltrans@{h i j k l} (l : TypeLevel) (wl : wfLCon) (Γ : context) (A : term)
+  (IA : IdRedTy@{i j k l} wl Γ l A)
+  (ih1 : forall wl' : wfLCon,
+      wl' ≤ε wl -> [LogRel@{i j k l} l | Γ ||- IdRedTy.ty@{i j k l} IA ]< wl' >)
+  (ih2 : forall (Δ : context) (wl' : wfLCon) (ρ : Δ ≤ Γ),
+      wl' ≤ε wl -> [ |-[ ta ] Δ ]< wl' > ->
+      forall wl'' : wfLCon,
+        wl'' ≤ε wl' ->
+        [LogRel@{i j k l} l | Δ ||- (IdRedTy.ty@{i j k l} IA)⟨ρ⟩ ]< wl'' >)
+  (wl' : wfLCon)
+  (f : wl' ≤ε wl)
+  (Hg : [ |-[ ta ] Γ ]< wl >) : IdRedTy@{i j k l} wl' Γ l A.
+Proof.
+  unshelve econstructor.
+  6: econstructor ; [eapply wft_Ltrans, (IdRedTy.red IA).(tyr_wf_r _ _ _ _) ; eauto |
+                      eapply redty_Ltrans ; eauto].
+  3: now eapply (IdRedTy.red IA).(tyr_wf_red _ _ _ _).
+  3: eapply convty_Ltrans ; eauto ; now eapply (IdRedTy.eq IA).
+  + now eapply ih1.
+  + intros * f' Hd ; eapply ih2 ; [ | eassumption | now eapply wfLCon_le_id].
+    now eapply wfLCon_le_trans.
+  + irrelevance0 ; [ now eapply (wk_id_ren_on Γ (IdRedTy.ty IA)) | ].
+    destruct (wk_id_ren_on Γ  (IdRedTy.lhs IA)). 
+    eapply (IdRedTy.tyKripkeTm IA wk_id _ _ (wfLCon_le_id _) f Hg (wfc_Ltrans f Hg)).
+    * now bsimpl.
+    * irrelevance0 ; [symmetry ; now eapply (wk_id_ren_on Γ (IdRedTy.ty IA)) | ].
+      now eapply (IdRedTy.lhsRed).
+  + irrelevance0 ; [ now eapply (wk_id_ren_on Γ (IdRedTy.ty IA)) | ].
+    destruct (wk_id_ren_on Γ  (IdRedTy.rhs IA)).
+    eapply (IdRedTy.tyKripkeTm IA wk_id _ _ (wfLCon_le_id _) f Hg (wfc_Ltrans f Hg)).
+    * now bsimpl.
+    * irrelevance0 ; [symmetry ; now eapply (wk_id_ren_on Γ (IdRedTy.ty IA)) | ].
+      now eapply (IdRedTy.rhsRed).
+  + irrelevance0 ; [ now eapply (wk_id_ren_on Γ (IdRedTy.ty IA)) | ].
+    destruct (wk_id_ren_on Γ  (IdRedTy.lhs IA)).
+    eapply (IdRedTy.tyKripkeTmEq IA wk_id _ _ (wfLCon_le_id _) f Hg (wfc_Ltrans f Hg)).
+    * now bsimpl.
+    * irrelevance0 ; [symmetry ; now eapply (wk_id_ren_on Γ (IdRedTy.ty IA)) | ].
+      now eapply (IdRedTy.lhsRedRefl).
+  + irrelevance0 ; [ now eapply (wk_id_ren_on Γ (IdRedTy.ty IA)) | ].
+    destruct (wk_id_ren_on Γ  (IdRedTy.rhs IA)).
+    eapply (IdRedTy.tyKripkeTmEq IA wk_id _ _ (wfLCon_le_id _) f Hg (wfc_Ltrans f Hg)).
+    * now bsimpl.
+    * irrelevance0 ; [symmetry ; now eapply (wk_id_ren_on Γ (IdRedTy.ty IA)) | ].
+      now eapply (IdRedTy.rhsRedRefl).
+  + econstructor.
+    * intros ??? ; eapply (LREqTermSymConv); [eassumption | ].
+      now eapply reflLRTyEq.
+    * intros ????? ; eapply (transEqTerm@{h i j k l}) ; eassumption.
+  + intros ?? wl'' wl''' ??? f' f'' ??? Heq Hyp.
+    irrelevance0 ; [reflexivity | ].
+    eapply (IdRedTy.tyKripkeEq IA _ _ _ (f' •ε f) f'' wfΔ wfΞ _ Heq).
+    irrelevance0 ; [ reflexivity | eassumption].
+  + intros ?? wl'' wl''' ??? f' f'' ??? Heq Hyp.
+    irrelevance0 ; [reflexivity | ].
+    eapply (IdRedTy.tyKripkeTm IA _ _ _ (f' •ε f) f'' wfΔ wfΞ _ Heq).
+    irrelevance0 ; [ reflexivity | eassumption].
+  + intros ?? wl'' wl''' ??? f' f'' ???? Heq Hyp.
+    irrelevance0 ; [reflexivity | ].
+    eapply (IdRedTy.tyKripkeTmEq IA _ _ _ (f' •ε f) f'' wfΔ wfΞ _ _ Heq).
+    irrelevance0 ; [ reflexivity | eassumption].
+Defined.
+
+  Lemma Ltrans@{h i j k l} {wl Γ wl' A l} :
+    (wl' ≤ε wl) ->
+    [LogRel@{i j k l} l | Γ ||- A]< wl > ->
+    [LogRel@{i j k l} l | Γ ||- A]< wl' >.
+  Proof.
+    intros f lrA. revert wl' f. pattern l, wl, Γ, A, lrA.
+    eapply LR_rect_TyUr@{i j k l l}; clear l wl Γ A lrA.
+    - intros * [??? []] ??. apply LRU_.
+      econstructor ; eauto ; [now eapply wfc_Ltrans | econstructor ].
+      + now eapply wft_Ltrans.
+      + now eapply redty_Ltrans.
+    - intros ????[ty[]]??. apply LRne_ ; econstructor ; [econstructor | ].
+      + now eapply wft_Ltrans.
+      + now eapply redty_Ltrans.
+      + now eapply convneu_Ltrans.
+    - intros ???? [] ihdom ihcod wl' f ; cbn in *.
+      apply LRPi' ; econstructor ; [destruct red ; econstructor |..].
+      + now eapply wft_Ltrans.
+      + now eapply redty_Ltrans.
+      + now eapply convty_Ltrans.
+      + now eapply convty_Ltrans.
+      + unshelve econstructor.
+        4,5: destruct polyRed ; now eapply wft_Ltrans.
+        * intros * f' Hd.
+          eapply (PolyRed.shpRed polyRed) ; [eapply wfLCon_le_trans | ] ; eauto.
+        * intros ???? f' Hd ha ; cbn in *.
+          eapply (PolyRed.posTree polyRed) ; eauto.
+        * intros ???? f' ??? Hover ; cbn in *.
+          eapply (PolyRed.posRed polyRed) ; eassumption.
+        * intros ???? f' ????? Hover Hover' ; cbn in *.
+          eapply (PolyRed.posExt polyRed) ; eassumption.
+    - intros ????? wl' f.
+      eapply LRNat_ ; econstructor.
+      eapply redtywf_Ltrans ; eauto.
+      now eapply NA.(NatRedTy.red).
+    - intros ????? wl' f.
+      eapply LRBool_ ; econstructor.
+      eapply redtywf_Ltrans ; eauto.
+      now eapply NA.(BoolRedTy.red).
+    - intros ????? wl' f.
+      eapply LREmpty_ ; econstructor.
+      eapply redtywf_Ltrans ; eauto.
+      now eapply NA.(EmptyRedTy.red).
+    - intros ???? [] ihdom ihcod wl' f ; cbn in *.
+      apply (LRSig'@{i j k l}) ; econstructor ; [destruct red ; econstructor |..].
+      + now eapply wft_Ltrans.
+      + now eapply redty_Ltrans.
+      + now eapply convty_Ltrans.
+      + now eapply convty_Ltrans.
+      + unshelve econstructor.
+        4,5: destruct polyRed ; now eapply wft_Ltrans.
+        * intros * f' Hd.
+          eapply (PolyRed.shpRed polyRed) ; [eapply wfLCon_le_trans | ] ; eauto.
+        * intros ???? f' Hd ha ; cbn in *.
+          eapply (PolyRed.posTree polyRed) ; eauto.
+        * intros ???? f' ??? Hover ; cbn in *.
+          eapply (PolyRed.posRed polyRed) ; eassumption.
+        * intros ???? f' ????? Hover Hover' ; cbn in *.
+          eapply (PolyRed.posExt polyRed) ; eassumption.
+    - intros ????? ih1 ih2 wl' f. 
+      apply (LRId'@{i j k l}).
+      eapply (Id_Ltrans@{h i j k l}) ; eauto.
+      now eapply (wfc_convty (IdRedTy.eq IA)).
+  Defined.
+
+  
+Lemma Eq_Ltrans@{h i j k l} {wl Γ wl' A B l} (f : wl' ≤ε wl) (lrA : [Γ ||-<l> A]< wl >) : 
+    [LogRel@{i j k l} l | Γ ||- A ≅ B | lrA]< wl > ->
+    [LogRel@{i j k l} l | Γ ||- A ≅ B | Ltrans@{h i j k l} f lrA]< wl' >.
+Proof.
+  revert B wl' f. pattern l, wl, Γ, A, lrA.
+  eapply LR_rect_TyUr@{i j k l l}; clear l wl Γ A lrA.
+  - intros ???? [??? []] ???[] ; cbn in *.
+    constructor ; constructor.
+    + now eapply wft_Ltrans.
+    + destruct red ; now eapply redty_Ltrans.
+  - intros ???? [?[]] ???[?[]] ; cbn in *.
+    econstructor ; [econstructor | ].
+    + now eapply wft_Ltrans.
+    + now eapply redty_Ltrans.
+    + now eapply convneu_Ltrans.
+  - intros ???? [] ihdom ihcod B wl' f []; cbn in *.
+    econstructor ; [destruct red0 ; econstructor |..].
+    + now eapply wft_Ltrans.
+    + now eapply redty_Ltrans.
+    + now eapply convty_Ltrans.
+    + now eapply convty_Ltrans.
+    + unshelve econstructor ; cbn in *.
+      * intros * ? ; now eapply (PolyRedEq.posTree polyRed0).
+      * intros * ; now eapply (PolyRedEq.shpRed polyRed0).
+      * cbn ; intros * Ho' ; now eapply (PolyRedEq.posRed polyRed0).
+  - intros ???? [[]] B wl' f [[]] ; cbn in *.
+    econstructor ; econstructor.
+    + now eapply wft_Ltrans.
+    + now eapply redty_Ltrans.
+  - intros ???? [[]] B wl' f [[]] ; cbn in *.
+    econstructor ; econstructor.
+    + now eapply wft_Ltrans.
+    + now eapply redty_Ltrans.
+  - intros ???? [[]] B wl' f [[]] ; cbn in *.
+    econstructor ; econstructor.
+    + now eapply wft_Ltrans.
+    + now eapply redty_Ltrans.
+  - intros ???? [] ihdom ihcod B wl' f [] ; cbn in *.
+    econstructor ; [destruct red0 ; econstructor | ..].
+    + now eapply wft_Ltrans.
+    + now eapply redty_Ltrans.
+    + now eapply convty_Ltrans.
+    + now eapply convty_Ltrans.
+    + unshelve econstructor ; cbn.
+      * intros * ? ; now eapply (PolyRedEq.posTree polyRed0).
+      * intros * ; now eapply (PolyRedEq.shpRed polyRed0).
+      * cbn ; intros * Ho' ; now eapply (PolyRedEq.posRed polyRed0).
+  - intros ????? ih1 ih2 ????.
+    assert (Hg:= (wfc_convty (IdRedTy.eq IA))).
+    eapply (@Build_IdRedTyEq _ _ _ _ _ _ wl' Γ A _ B) ; cbn.
+    + unshelve econstructor.
+      * now eapply wft_Ltrans, (IdRedTyEq.red X).(tyr_wf_r _ _ _ _).
+      * now eapply redty_Ltrans, (IdRedTyEq.red X).(tyr_wf_red _ _ _ _).
+    + eapply convty_Ltrans ; [ eassumption | ].
+      eapply (IdRedTyEq.eq X). 
+    + eapply ih1.
+      now eapply (IdRedTyEq.tyRed X).
+    + irrelevance0 ; [ now eapply (wk_id_ren_on Γ (IdRedTy.ty IA)) | ].
+      destruct (wk_id_ren_on Γ  (IdRedTy.lhs IA)).
+      destruct (wk_id_ren_on Γ  (IdRedTyEq.lhs X)).
+      eapply (IdRedTy.tyKripkeTmEq IA wk_id _ _ (wfLCon_le_id _) f Hg (wfc_Ltrans f Hg)).
+      * now bsimpl.
+      * irrelevance0 ; [ symmetry ; now eapply (wk_id_ren_on Γ (IdRedTy.ty IA)) | ].
+        exact (IdRedTyEq.lhsRed X).
+    + irrelevance0 ; [ now eapply (wk_id_ren_on Γ (IdRedTy.ty IA)) | ].
+      destruct (wk_id_ren_on Γ  (IdRedTy.rhs IA)).
+      destruct (wk_id_ren_on Γ  (IdRedTyEq.rhs X)).
+      eapply (IdRedTy.tyKripkeTmEq IA wk_id _ _ (wfLCon_le_id _) f Hg (wfc_Ltrans f Hg)).
+      * now bsimpl.
+      * irrelevance0 ; [ symmetry ; now eapply (wk_id_ren_on Γ (IdRedTy.ty IA)) | ].
+        exact (IdRedTyEq.rhsRed X).
+Qed.
+
+
+Lemma isLRFun_Ltrans : forall wl wl' Γ t A l (f : wl' ≤ε wl) (ΠA : [Γ ||-Π< l > A]< wl >)
+                              (ΠA' : [Γ ||-Π< l > A]< wl' >),
+    isLRFun ΠA t -> isLRFun ΠA' t.
+Proof.
+  intros * f * Hyp.
+  unshelve epose (Heq := redtywf_det _ _ (redtywf_Ltrans f ΠA.(ParamRedTyPack.red)) ΠA'.(ParamRedTyPack.red)).
+  1,2: now econstructor.
+  inversion Heq.
+  induction Hyp as [?? funTree e r | t Heqt].
+  - unshelve econstructor.
+    + intros Δ wl'' a ρ f' Hd ha ; cbn.
+      eapply DTree_fusion.
+      * unshelve eapply funTree.
+        6: irrelevance0 ; [ | exact ha] ; now f_equal.
+        2: assumption.
+        now eapply wfLCon_le_trans.
+      * unshelve eapply (PolyRedPack.posTree ΠA).
+        5: eassumption.
+        4: irrelevance0 ; [ | exact ha] ; now f_equal.
+        now eapply wfLCon_le_trans.
+    + intros Δ wl'' ρ f' Hd ; cbn.
+      irrelevance0 ; [ | unshelve eapply e] ; [now f_equal | ..].
+      2: assumption.
+      now eapply wfLCon_le_trans.
+    + intros Δ wl'' a ρ f' Hd ha wl''' Ho Ho'.
+      irrelevance0 ; [ | unshelve eapply r].
+      now f_equal.
+      3: eassumption.
+      now eapply wfLCon_le_trans.
+      cbn in *.
+      3: now eapply over_tree_fusion_l.
+      now eapply over_tree_fusion_r.
+  - econstructor 2.
+    cbn in *.
+    rewrite <- H11, <- H12.
+    now eapply convneu_Ltrans.
+Qed.
+
+Lemma isLRPair_Ltrans : forall wl wl' Γ t A l (f : wl' ≤ε wl) (ΣA : [Γ ||-Σ< l > A]< wl >)
+                              (ΣA' : [Γ ||-Σ< l > A]< wl' >),
+    isLRPair ΣA t -> isLRPair ΣA' t.
+Proof.
+  intros * f * Hyp.
+  unshelve epose (Heq := redtywf_det _ _ (redtywf_Ltrans f ΣA.(ParamRedTyPack.red)) ΣA'.(ParamRedTyPack.red)).
+  1,2: now econstructor.
+  inversion Heq.
+  induction Hyp as [????? fstTree ?? sndTree | t Heqt].
+  - unshelve econstructor.
+    + intros Δ wl'' a' ρ f' Hd ha ; cbn.
+      eapply DTree_fusion.
+      * unshelve eapply fstTree.
+        6: irrelevance0 ; [ | exact ha] ; now f_equal.
+        2: assumption.
+        now eapply wfLCon_le_trans.
+      * unshelve eapply (PolyRedPack.posTree ΣA).
+        5: eassumption.
+        4: irrelevance0 ; [ | exact ha] ; now f_equal.
+        now eapply wfLCon_le_trans.
+    + intros Δ wl'' ρ f' Hd ; cbn.
+      irrelevance0 ; [ | unshelve eapply rfst] ; [now f_equal | ..].
+      2: assumption.
+      now eapply wfLCon_le_trans.
+    + intros Δ wl'' ρ f' Hd.
+      eapply DTree_fusion.
+      * eapply sndTree.
+        1,3: eassumption.
+        now eapply wfLCon_le_trans.
+      * unshelve  eapply (PolyRed.posTree ΣA).
+        6: now unshelve eapply rfst.
+        2,4: eassumption.
+        now eapply wfLCon_le_trans.
+    + intros Δ wl'' ρ f' Hd.
+      irrelevance0 ; [ | unshelve eapply rdom ; eauto].
+      now f_equal.
+      now eapply wfLCon_le_trans.
+    + intros Δ wl'' a' ρ f' Hd ha wl''' Ho Ho' ; cbn in *.
+      irrelevance0 ; [ | unshelve eapply rcod].
+      1: now f_equal.
+      3: eassumption.
+      * now eapply wfLCon_le_trans.
+      * irrelevance0 ; [ | exact ha] ; now f_equal.
+      * cbn in * ; now eapply over_tree_fusion_r.
+      * cbn in * ; now eapply over_tree_fusion_l.
+    + intros Δ wl'' ρ f' Hd wl''' Ho Ho' ; cbn in *.
+      irrelevance0 ; [ | unshelve eapply rsnd].
+      1: now f_equal.
+      3: eassumption.
+      * now eapply wfLCon_le_trans.
+      * cbn in * ; now eapply over_tree_fusion_r.
+      * cbn in * ; now eapply over_tree_fusion_l.
+  - econstructor 2.
+    cbn in *.
+    rewrite <- H11, <- H12.
+    now eapply convneu_Ltrans.
+Qed.
+
+Lemma NatTm_Ltrans (l : TypeLevel) (wl : wfLCon) (Γ : context) (A : term)
+  (NA : [Γ ||-Nat A ]< wl >) (t : term) (wl' : wfLCon) (f : wl' ≤ε wl) (NA' : [Γ ||-Nat A ]< wl' >) :
+  [LRNat_ l NA | Γ ||- t : A ]< wl > -> [ (LRNat_ l NA') | Γ ||- t : A ]< wl' >.
+Proof.
+  revert t.
+  set (G := _); enough (h : G × (forall t, NatProp NA t -> NatProp NA' t)) by apply h.
+  subst G; apply NatRedInduction.
+  - intros t nf Hred Heq Hprop Hprop'.
+    econstructor ; [now eapply redtmwf_Ltrans | | ].
+    + now eapply convtm_Ltrans.
+    + assumption.
+  - now econstructor.
+  - intros n Hn Hn' ; now econstructor.
+  - intros ; econstructor.
+    destruct r ; econstructor.
+    + now eapply ty_Ltrans.
+    + now eapply convneu_Ltrans.
+Qed.
+
+Lemma IdTm_Ltrans (l : TypeLevel) (wl wl' : wfLCon) (Γ : context) (A : term) (f : wl' ≤ε wl)
+  (IA : [Γ ||-Id< l > A ]< wl >) (IA' : [Γ ||-Id< l > A ]< wl' >)
+  (ih1 : forall (t : term),
+      [IdRedTy.tyRed IA | Γ ||- t : IdRedTy.ty IA ]< wl > ->
+      [IdRedTy.tyRed IA' | Γ ||- t : IdRedTy.ty IA' ]< wl' >)
+  (ih2 : forall (Δ : context) (ρ : Δ ≤ Γ) (wfΔ : [ |-[ ta ] Δ ]< wl' >)
+                (t : term) (wl'' : wfLCon) (f' : wl'' ≤ε wl'),
+      [IdRedTy.tyKripke IA ρ f wfΔ | Δ ||- t : (IdRedTy.ty IA)⟨ρ⟩ ]< wl' > ->
+      [IdRedTy.tyKripke IA' ρ f' (wfc_Ltrans f' wfΔ) | Δ ||- t : (IdRedTy.ty IA')⟨ρ⟩ ]< wl'' >) :
+      forall (t : term),
+        [LRId' IA | Γ ||- t : A ]< wl > -> [LRId' IA' | Γ ||- t : A ]< wl' >.
+Proof.
+  intros t Ht.
+  unshelve epose (Heq := redtywf_det _ _ (redtywf_Ltrans f (IdRedTy.red IA))
+                           (IdRedTy.red IA')).
+  1,2 : now econstructor.
+  inversion Heq.
+  assert (Hg:= (wfc_convty (IdRedTy.eq IA))).
+  econstructor ; cbn.
+  - cbv in H11,H12,H13 ; cbv. 
+    rewrite <- H11, <- H12, <- H13.
+    now eapply redtmwf_Ltrans ; [ | eapply (IdRedTm.red Ht)].
+  - cbv in H11,H12,H13 ; cbv. 
+    rewrite <- H11, <- H12, <- H13.
+    now eapply convtm_Ltrans ; [ | eapply (IdRedTm.eq Ht)].
+  - destruct (IdRedTm.prop Ht).
+    + econstructor.
+      * now eapply wft_Ltrans.
+      * now eapply ty_Ltrans.
+      * irrelevance0 ; [ | unshelve eapply Eq_Ltrans].
+        5: eassumption.
+        all: assumption.
+      * assert (Help : IdRedTyPack.lhs (IdRedTy.toPack IA') = IdRedTyPack.lhs (IdRedTy.toPack IA)).
+        { now eauto. }
+        rewrite Help.
+        irrelevance0.
+        2:{ erewrite <- (wk_id_ren_on Γ (IdRedTyPack.lhs (IdRedTy.toPack IA))).
+            erewrite <- wk_id_ren_on.
+            eapply (IdRedTy.tyKripkeTmEq IA wk_id wk_id _ (wfLCon_le_id _) f Hg (wfc_Ltrans f Hg)).
+            * now bsimpl.
+            * irrelevance0 ; [rewrite wk_id_ren_on ; reflexivity | ].
+              eassumption.
+        }
+        rewrite H11 ; bsimpl.
+        reflexivity.
+      * assert (Help : IdRedTyPack.rhs (IdRedTy.toPack IA') = IdRedTyPack.rhs (IdRedTy.toPack IA)).
+        { now eauto. }
+        rewrite Help.
+        irrelevance0.
+        2:{ erewrite <- (wk_id_ren_on Γ (IdRedTyPack.rhs (IdRedTy.toPack IA))).
+            erewrite <- wk_id_ren_on.
+            eapply (IdRedTy.tyKripkeTmEq IA wk_id wk_id _ (wfLCon_le_id _) f Hg (wfc_Ltrans f Hg)).
+            * now bsimpl.
+            * irrelevance0 ; [rewrite wk_id_ren_on ; reflexivity | ].
+              eassumption.
+        }
+        rewrite H11 ; bsimpl.
+        reflexivity.
+    + econstructor.
+      destruct r ; econstructor.
+      * eapply ty_Ltrans ; [eassumption | ].
+        assert (Help : IdRedTyPack.outTy (IdRedTy.toPack IA') = IdRedTyPack.outTy (IdRedTy.toPack IA)) by eauto.
+        now rewrite Help.
+      * eapply convneu_Ltrans ; [eassumption | ].
+        assert (Help : IdRedTyPack.outTy (IdRedTy.toPack IA') = IdRedTyPack.outTy (IdRedTy.toPack IA)) by eauto.
+        now rewrite Help.
+Qed.
+
+Lemma ΠTm_Ltrans (l : TypeLevel) (wl wl' : wfLCon) (Γ : context) (f : wl' ≤ε wl) (A : term)
+  (ΠA : [Γ ||-Π< l > A ]< wl >)
+  (ΠA' : [Γ ||-Π< l > A ]< wl' >)
+  (ihdom : forall (Δ : context) (ρ : Δ ≤ Γ) (h : [ |-[ ta ] Δ ]< wl' >) (t : term)
+                  (wl'' : wfLCon) (f' : wl'' ≤ε wl'),
+      [PolyRed.shpRed ΠA ρ f h | Δ ||- t : (ParamRedTy.dom ΠA)⟨ρ⟩ ]< wl' > ->
+      [Ltrans f' (PolyRed.shpRed ΠA ρ f h) | Δ ||- t : (ParamRedTy.dom ΠA)⟨ρ⟩ ]< wl'' >)
+  (ihcod : forall (Δ : context) (a : term) (ρ : Δ ≤ Γ) (h : [ |-[ ta ] Δ ]< wl' >)
+                  (ha : [PolyRed.shpRed ΠA ρ f h | Δ ||- a : (ParamRedTy.dom ΠA)⟨ρ⟩ ]< wl' >)
+                  (wl'' : wfLCon) (Ho : over_tree wl' wl'' (PolyRed.posTree ΠA ρ f h ha))
+                  (t : term) (wl''' : wfLCon) (f'' : wl''' ≤ε wl''),
+      [PolyRed.posRed ΠA ρ f h ha Ho | Δ  ||- t : (ParamRedTy.cod ΠA)[a .: ρ >> tRel] ]< wl'' > ->
+      [Ltrans f'' (PolyRed.posRed ΠA ρ f h ha Ho) | Δ  ||- t : (ParamRedTy.cod ΠA)[a .: ρ >> tRel] ]< wl''' >) :
+  forall (t : term),
+    [Γ ||-Π t : A | ΠA ]< wl > ->  [Γ ||-Π t : A | ΠA' ]< wl' >.
+Proof.
+  intros t [].
+  unshelve econstructor ; [ | | eapply redtmwf_Ltrans ; eauto |..].
+  1: exact nf.
+  1:{ cbn in * ; intros.
+      eapply DTree_fusion.
+      * unshelve eapply appTree.
+        4: eapply wfLCon_le_trans.
+        3-6: eassumption.
+        2: irrelevance0 ; [ | eassumption ].
+        f_equal.
+        unshelve epose (Heq := redtywf_det _ _ (redtywf_Ltrans f ΠA.(ParamRedTyPack.red)) ΠA'.(ParamRedTyPack.red)) ; [now econstructor | now econstructor | ].
+        now inversion Heq.
+    * eapply (PolyRed.posTree ΠA ρ (f0 •ε f) Hd).
+      irrelevance0 ; [ | eassumption].
+      f_equal.
+      unshelve epose (Heq := redtywf_det _ _ (redtywf_Ltrans f ΠA.(ParamRedTyPack.red)) ΠA'.(ParamRedTyPack.red)) ; [now econstructor | now econstructor | ].
+      now inversion Heq.
+  }
+  all: unshelve epose (Heq := redtywf_det _ _ (redtywf_Ltrans f ΠA.(ParamRedTyPack.red)) ΠA'.(ParamRedTyPack.red)) ; [now econstructor | now econstructor | ].
+  all: inversion Heq.
+  2: eapply convtm_Ltrans ; [eauto | now rewrite <- Heq].
+  2: eapply isLRFun_Ltrans ; eauto.
+  1: now rewrite <- Heq.
+  + cbn in * ; intros. 
+    irrelevance0 ; [ | unshelve eapply app].
+    6: now eapply over_tree_fusion_r.
+    * now f_equal.
+    * now eapply over_tree_fusion_l.
+  + cbn in * ; intros.
+    irrelevance0 ; [ | unshelve eapply eq].
+    9: now eapply over_tree_fusion_l.
+    2: now eapply over_tree_fusion_r.
+    1: now f_equal.
+    1,2: irrelevance0 ; [ | eassumption] ; now f_equal.
+Defined.
+
+Lemma ΣTm_Ltrans (l : TypeLevel) (wl wl' : wfLCon) (Γ : context) (f : wl' ≤ε wl) (A : term)
+  (ΣA : [Γ ||-Σ< l > A ]< wl >)
+  (ΣA' : [Γ ||-Σ< l > A ]< wl' >)
+  (ihdom : forall (Δ : context) (ρ : Δ ≤ Γ) (h : [ |-[ ta ] Δ ]< wl' >) (t : term)
+                  (wl'' : wfLCon) (f' : wl'' ≤ε wl'),
+      [PolyRed.shpRed ΣA ρ f h | Δ ||- t : (ParamRedTy.dom ΣA)⟨ρ⟩ ]< wl' > ->
+      [Ltrans f' (PolyRed.shpRed ΣA ρ f h) | Δ ||- t : (ParamRedTy.dom ΣA)⟨ρ⟩ ]< wl'' >)
+  (ihcod : forall (Δ : context) (a : term) (ρ : Δ ≤ Γ) (h : [ |-[ ta ] Δ ]< wl' >)
+                  (ha : [PolyRed.shpRed ΣA ρ f h | Δ ||- a : (ParamRedTy.dom ΣA)⟨ρ⟩ ]< wl' >)
+                  (wl'' : wfLCon) (Ho : over_tree wl' wl'' (PolyRed.posTree ΣA ρ f h ha))
+                  (t : term) (wl''' : wfLCon) (f'' : wl''' ≤ε wl''),
+      [PolyRed.posRed ΣA ρ f h ha Ho | Δ  ||- t : (ParamRedTy.cod ΣA)[a .: ρ >> tRel] ]< wl'' > ->
+      [Ltrans f'' (PolyRed.posRed ΣA ρ f h ha Ho) | Δ  ||- t : (ParamRedTy.cod ΣA)[a .: ρ >> tRel] ]< wl''' >) :
+  forall (t : term),
+    [Γ ||-Σ t : A | ΣA ]< wl > ->  [Γ ||-Σ t : A | ΣA' ]< wl' >.
+Proof.
+  intros t [].
+  unshelve econstructor.
+  4: eapply redtmwf_Ltrans ; eauto.
+  1: exact nf.
+  2:{ cbn in * ; intros.
+      eapply DTree_fusion.
+      * unshelve eapply sndTree.
+        3: eapply wfLCon_le_trans.
+        2-5: eassumption.
+      * eapply (PolyRed.posTree ΣA ρ (f0 •ε f) Hd).
+        eapply fstRed.
+  }
+  all: unshelve epose (Heq := redtywf_det _ _ (redtywf_Ltrans f ΣA.(ParamRedTyPack.red)) ΣA'.(ParamRedTyPack.red)) ; [now econstructor | now econstructor | ].
+  all: inversion Heq.
+  3: eapply convtm_Ltrans ; [eauto | ].
+  2,3: cbv ; cbv in Heq ; now rewrite <- Heq.
+  2: eapply isLRPair_Ltrans ; now eauto.
+  + cbn in * ; intros.
+    irrelevance0 ; [ | unshelve eapply fstRed].
+    * now f_equal.
+    * now eapply wfLCon_le_trans.
+    * assumption.
+  + cbn in * ; intros.
+    irrelevance0 ; [ | unshelve eapply sndRed].
+    4: eassumption.
+    * now f_equal.
+    * now eapply wfLCon_le_trans.
+    * now eapply over_tree_fusion_r.
+    * now eapply over_tree_fusion_l.
+Defined.
+  
+Lemma Tm_Ltrans@{h i j k l} {wl Γ wl' t A l} (f : wl' ≤ε wl) (lrA : [Γ ||-<l> A]< wl >) : 
+    [LogRel@{i j k l} l | Γ ||- t : A | lrA]< wl > ->
+    [LogRel@{i j k l} l | Γ ||- t : A | Ltrans@{h i j k l} f lrA]< wl' >.
+Proof.
+  revert t wl' f. pattern l, wl, Γ, A, lrA.
+  eapply LR_rect_TyUr@{i j k l l}; clear l wl Γ A lrA.
+  - intros ???? [??? []] ???[?[]].
+    econstructor ; [ econstructor | eassumption |.. ].
+    + now eapply ty_Ltrans.
+    + now eapply redtm_Ltrans.
+    + now eapply convtm_Ltrans.
+    + apply RedTyRecBwd ; apply RedTyRecFwd in rel.
+      now eapply Ltrans ; eauto.
+  - intros ???? [?[]] ???[?[]] ; cbn in *.
+    econstructor ; [econstructor ; cbn | ].
+    + now eapply ty_Ltrans.
+    + now eapply redtm_Ltrans.
+    + now eapply convneu_Ltrans.
+  - intros ???? [] ihdom ihcod t wl' f ?.
+    cbn in *.
+    unshelve eapply ΠTm_Ltrans ; intros.
+    6: eassumption.
+    1: eassumption.
+    + now eapply ihdom.
+    + now eapply ihcod. 
+  - intros ; irrelevance0 ; [ reflexivity | unshelve eapply NatTm_Ltrans].
+    5: eassumption.
+    2: assumption.
+    destruct NA ; econstructor ; now eapply redtywf_Ltrans.
+  - intros ???? NA t ? f ; revert t ; cbn.
+    intros t Ht. induction Ht. econstructor.
+    + now eapply redtmwf_Ltrans.
+    + now eapply convtm_Ltrans.
+    + destruct prop as [ | | m Hne] ; econstructor.
+      destruct Hne ; econstructor.
+      * now eapply ty_Ltrans.
+      * now eapply convneu_Ltrans.
+  - intros ???? NA t ? f Ht ; cbn.
+    induction Ht ; econstructor.
+    + now eapply redtmwf_Ltrans.
+    + now eapply convtm_Ltrans.
+    + destruct prop as [m Hne] ; econstructor.
+      destruct Hne ; econstructor.
+      * now eapply ty_Ltrans.
+      * now eapply convneu_Ltrans.
+  - intros ????? ihdom ihcod t wl' f ?; cbn in *.
+    eapply ΣTm_Ltrans.
+    + intros ; eauto.
+    + intros ; eauto.
+    + assumption.
+      Unshelve. assumption.
+  - intros * ih1 ih2 *.
+    unshelve eapply IdTm_Ltrans.
+    eassumption.
+    + intros ; eapply ih1 ; auto.
+    + intros ; eapply ih2.
+      rewrite <- (wk_id_ren_on Δ t0).
+      eapply (IdRedTy.tyKripkeTm IA ρ).
+      * now bsimpl.
+      * eassumption.
+Qed.
+
+Lemma TmEq_Ltrans@{h i j k l} {wl Γ wl' t u A l} (f : wl' ≤ε wl) (lrA : [Γ ||-<l> A]< wl >) : 
+    [LogRel@{i j k l} l | Γ ||- t ≅ u : A | lrA]< wl > ->
+    [LogRel@{i j k l} l | Γ ||- t ≅ u : A | Ltrans@{h i j k l} f lrA]< wl' >.
+Proof.
+  revert t u wl' f. pattern l, wl, Γ, A, lrA.
+  eapply LR_rect_TyUr@{i j k l l}; clear l wl Γ A lrA.
+  - intros ???? [??? []] ???? [].
+    unshelve econstructor.
+    + destruct redL.
+      econstructor.
+      * now eapply redtmwf_Ltrans.
+      * assumption.
+      * now eapply convtm_Ltrans.
+      * apply RedTyRecBwd ; clear relEq ; apply RedTyRecFwd in relL.
+        now eapply Ltrans.
+    + destruct redR.
+      econstructor.
+      * now eapply redtmwf_Ltrans.
+      * assumption.
+      * now eapply convtm_Ltrans.
+      * apply RedTyRecBwd ; clear relEq ; apply RedTyRecFwd in relR.
+        now eapply Ltrans.
+    + apply RedTyRecBwd ; clear relEq ; apply RedTyRecFwd in relL.
+      now eapply Ltrans.
+    + cbn in *.
+      now eapply convtm_Ltrans.
+    + apply RedTyRecBwd ; clear relEq ; apply RedTyRecFwd in relR.
+      now eapply Ltrans.
+    + eapply TyEqRecBwd, Eq_Ltrans ; cbn.
+      now eapply TyEqRecFwd.
+  - intros ???? [?[]] ???? [] ; cbn in *.
+    econstructor.
+    + now eapply redtmwf_Ltrans.
+    + now eapply redtmwf_Ltrans.
+    + now eapply convneu_Ltrans.
+  - intros ????? ihdom ihcod t u wl' f [].
+    cbn.
+    unshelve econstructor ; cbn in *.
+    + unshelve eapply ΠTm_Ltrans ; [ | eassumption | ..].
+      1,4: eassumption.
+      * intros ; now eapply Tm_Ltrans.
+      * intros ; now eapply Tm_Ltrans.
+    + unshelve eapply ΠTm_Ltrans ; [ | eassumption | ..].
+      1,4: eassumption.
+      * intros ; now eapply Tm_Ltrans.
+      * intros ; now eapply Tm_Ltrans.
+    + intros ; eapply eqTree.
+      eassumption.
+    + intros ; cbn in *.
+      now eapply convtm_Ltrans.
+    + intros ; cbn in *.
+      eapply eqApp.
+      assumption.
+  - intros * ; revert t u.
+    set (NA' := {| NatRedTy.red := redtywf_Ltrans f (NatRedTy.red NA) |}).
+    set (G := _); enough (h : G × (forall t u, NatPropEq NA t u -> NatPropEq NA' t u)) by apply h.
+    subst G; apply NatRedEqInduction.
+    + intros t u nt nu Hredt Hredu Heq Hprop Hprop'.
+      econstructor.
+      1,2: now eapply redtmwf_Ltrans.
+      * now eapply convtm_Ltrans.
+      * assumption.
+    + now econstructor.
+    + intros n Hn Hn' ; now econstructor.
+    + intros ; econstructor.
+      destruct r ; econstructor.
+      now eapply convneu_Ltrans.
+  - intros ???? NA t ? wl' f Heq.
+    induction Heq ; cbn. econstructor.
+    1,2: now eapply redtmwf_Ltrans.
+    + now eapply convtm_Ltrans.
+    + destruct prop as [ | | m Hne] ; econstructor.
+      econstructor.
+      now destruct r ; eapply convneu_Ltrans.
+  - intros ???? NA t u wl' f Heq ; cbn.
+    induction Heq ; econstructor.
+    1,2: now eapply redtmwf_Ltrans.
+    + now eapply convtm_Ltrans.
+    + destruct prop as [m Hne] ; econstructor ; econstructor.
+      now destruct r ; eapply convneu_Ltrans.
+  - cbn ; intros ????? ihdom ihcod t u wl' f []; cbn in *.
+    unshelve econstructor ; cbn.
+    + unshelve eapply ΣTm_Ltrans.
+      2,3,6: eassumption.
+      * intros.
+        irrelevance0 ; [ | unshelve eapply Tm_Ltrans].
+        5: eassumption.
+        1,2: now auto.
+      * intros.
+        irrelevance0 ; [ | unshelve eapply Tm_Ltrans].
+        5: eassumption.
+        1,2: now trivial.
+    + unshelve eapply ΣTm_Ltrans.
+      2,3,6: eassumption.
+      * intros.
+        irrelevance0 ; [ | unshelve eapply Tm_Ltrans].
+        5: eassumption.
+        1,2: now auto.
+      * intros.
+        irrelevance0 ; [ | unshelve eapply Tm_Ltrans].
+        5: eassumption.
+        1,2: now trivial.
+    + intros ; eapply DTree_fusion.
+      * eapply eqTree.
+        1,3: eassumption.
+        now eapply wfLCon_le_trans.
+      * eapply (PolyRed.posTree ΠA ρ (f0 •ε f) Hd).
+        now eapply (SigRedTm.fstRed redL). 
+    + cbn ; now eapply convtm_Ltrans.
+    + cbn ; intros ; now unshelve eapply eqFst.
+    + cbn in * ; intros.
+      irrelevance0 ; [ reflexivity | unshelve eapply eqSnd].
+      3: eassumption.
+      * now eapply wfLCon_le_trans.
+      * now eapply over_tree_fusion_r.
+      * now eapply over_tree_fusion_l.
+  - intros ????? ih1 ih2 ???? [].
+    unshelve econstructor ; cbn.
+    3,4: now eapply redtmwf_Ltrans.
+    1: now eapply convtm_Ltrans.
+    destruct prop.
+    + econstructor.
+      1,2: now eapply wft_Ltrans.
+      1,2: now eapply ty_Ltrans.
+      1,2:irrelevance0 ; [ | now eapply Eq_Ltrans] ; reflexivity.
+      all: now eapply ih1.
+    + econstructor.
+      destruct r ; econstructor.
+      now eapply convneu_Ltrans.
+      Unshelve. all: assumption.
+Qed.
+  
+End Red_Ltrans.
